work on congress tests

execution/theories/CongressTests.v
@@ -13,11 +13,10 @@ From Coq Require Import Morphisms.
 From Coq Require Import Program.Basics.
 Import ListNotations.
 Notation "f 'o' g" := (compose f g) (at level 50).
-
 (* Generators for the types defined in the Congress contract *)
-
-Let BaseTypes := LocalChainBase AddrSize.
-Example ca : @CongressAction BaseTypes := cact_transfer zero_address 0%Z.
+Definition LocalChainBase : ChainBase := Generators.LocalChainBase.
+(* Let LocalBaseTypes := LocalChainBase AddrSize. *)
+Example ca : @CongressAction LocalChainBase := cact_transfer zero_address 0%Z.
 Open Scope string_scope.
 
 Instance showRules : Show Rules :=
@@ -55,7 +54,7 @@ Instance showSetup : Show Setup :=
     show := show o setup_rules
   |}.
 
-Definition string_of_Msg (m : Msg) : string :=
+Definition string_of_Msg `{Show SerializedValue} (m : @Msg LocalChainBase) : string :=
   match m with
     | transfer_ownership addr => "(transfer_ownership " ++  show addr ++ ")"
     | change_rules rules => "(change_rules " ++ show rules ++ ")"
@@ -68,15 +67,31 @@ Definition string_of_Msg (m : Msg) : string :=
     | finish_proposal proposalId => "(finish_proposal " ++ show proposalId ++ ")"
   end.
 
-Instance showMsg : Show Msg :=
+Instance showMsg `{Show SerializedValue} : Show (@Msg LocalChainBase) :=
 {|
   show := string_of_Msg
 |}.
 
-Close Scope string_scope.
+
+(* Generators *)
+
+(* Helpers for ChainContext *)
+Definition ctx_gAccountAddr (ctx : ChainContext LocalChainBase) : G (@Address LocalChainBase) := 
+  @gInvalidContractAddr LocalChainBase ctx.
+Definition ctx_gContractAddr (ctx : ChainContext LocalChainBase) : G (@Address LocalChainBase) := 
+  @gValidContractAddr LocalChainBase ctx.
+Definition ctx_gAnyAddr (ctx : ChainContext LocalChainBase) : G (@Address LocalChainBase) := 
+  @gAddress LocalChainBase ctx.
+Definition ctx_accounts (ctx : ChainContext LocalChainBase) : list Address := 
+  @accounts LocalChainBase ctx.
+Definition ctx_contracts (ctx : ChainContext LocalChainBase) : list Address := 
+  @contracts LocalChainBase ctx.
+
+Definition gZPositive := liftM Z.of_nat arbitrary.
+Definition gZPositiveSized n := liftM Z.of_nat (arbitrarySized n).
 
 Definition gRulesSized (n : nat) : G Rules :=
-  vote_count <- arbitrarySized n ;;
+  vote_count <- gZPositiveSized n ;;
   margin <- liftM Z.of_nat (gIntervalNat n (2 * n)) ;;
   liftM (build_rules vote_count margin) arbitrary.  
 
@@ -85,33 +100,68 @@ Instance genRulesSized : GenSized Rules :=
     arbitrarySized := gRulesSized
   |}.
 
+Instance genSetupSized : GenSized Setup := 
+{|
+  arbitrarySized n := liftM build_setup (arbitrarySized n)
+|}.
 
-Definition gCongressAction {ctx : ChainContext BaseTypes}
+
+
+Definition gCongressAction' {ctx : ChainContext LocalChainBase}
                            (gMsg : G SerializedValue) 
                            : G CongressAction :=
-  let gAddr := (gInvalidContractAddr BaseTypes ctx) in
+  (* We only want to generate positive amounts for now, but could be worth looking into *)
   freq [
-    (1, liftM2 cact_transfer gAddr arbitrary);
-    (1, liftM3 cact_call gAddr arbitrary gMsg)
+    (1, liftM2 cact_transfer (ctx_gAccountAddr ctx) gZPositive);
+    (1, liftM3 cact_call (ctx_gContractAddr ctx) gZPositive gMsg)
   ].
+Sample (ctx <- @arbitrarySized _ genLocalBaseGens 1 ;; @gCongressAction' ctx arbitrary).
 
-Fixpoint gMsgSized {ctx : ChainContext BaseTypes} (n : nat) : G Msg :=
-  let nonrec_gens := [
-      (1, liftM transfer_ownership (gInvalidContractAddr _ ctx)) ;
-      (1, liftM change_rules arbitrary) ;
-      (1, liftM add_member (gInvalidContractAddr _ ctx)) ;
-      (1, liftM remove_member (gInvalidContractAddr _ ctx)) ;
-      (1, liftM vote_for_proposal arbitrary) ;
-      (1, liftM vote_against_proposal arbitrary) ;
-      (1, liftM retract_vote arbitrary) ;
-      (1, liftM finish_proposal arbitrary)
-    ] in 
-  let default := liftM transfer_ownership (gInvalidContractAddr _ ctx) in
+
+
+Definition gMsgSimple (ctx : ChainContext LocalChainBase) : G Msg := 
+  freq [
+    (1, liftM transfer_ownership (ctx_gAccountAddr ctx)) ;
+    (1, liftM change_rules arbitrary) ;
+    (2, liftM add_member (ctx_gAccountAddr ctx)) ;
+    (2, liftM remove_member (ctx_gAccountAddr ctx)) ;
+    (2, liftM vote_for_proposal arbitrary) ;
+    (2, liftM vote_against_proposal arbitrary) ;
+    (2, liftM retract_vote arbitrary) ;
+    (2, liftM finish_proposal arbitrary)
+  ].
+Definition gMsg' : G Msg := 
+  ctx <- arbitrary ;; gMsgSimple ctx.
+
+Sample gMsg'.
+
+
+Sample (ctx <- @arbitrarySized _ genLocalBaseGens 1 ;; @gInvalidContractAddr LocalChainBase ctx).
+
+
+Fixpoint gMsgSized (ctx : ChainContext LocalChainBase) (n : nat) : G Msg :=
+  let default := liftM transfer_ownership (ctx_gAccountAddr ctx) in
   match n with
-    | 0 => (freq_ default nonrec_gens)
-    | S n' =>
-    let rec_gens := 
-      (1, liftM create_proposal (listOf (@gCongressAction ctx (liftM serialize (@gMsgSized ctx n')))))
-      :: nonrec_gens in
-    freq_ default rec_gens
+    | 0 => gMsgSimple ctx
+    | S n' => freq [
+        (1, (* TODO: fix weight. should be roughly 1:8*)
+        (* recurse. Msg is converted to a SerializedType using 'serialize' *)
+        (* This makes it possible to create proposals about proposals about proposals etc... *)
+        congressActions <- listOf (@gCongressAction' ctx (liftM serialize (gMsgSized ctx n'))) ;;
+        returnGen (create_proposal congressActions)) ;
+        (1, gMsgSimple ctx)
+      ]
   end.
+
+Sample (ctx <- arbitrary ;; @gMsgSized ctx 4).
+
+Definition gCongressActionSized {ctx : ChainContext LocalChainBase}
+                                (n : nat)
+                                : G CongressAction := @gCongressAction' ctx (liftM serialize (@gMsgSized ctx n)).
+
+
+Sample (ctx <- arbitrary ;; gMsgSized ctx 3).
+
+Example ex_call_congress_action := ctx <- arbitrary ;; liftM (cact_call zero_address 0%Z) (liftM serialize (gMsgSized ctx 3) ).
+Sample ex_call_congress_action.
+Close Scope string_scope.
